x86/Asmgenproof1.v
@@ -1431,11 +1431,7 @@ Transparent destroyed_by_op.
   rewrite Pregmap.gss. rewrite <- EV; auto.
   intros; Simplifs.
   TranslOp. rewrite nextinstr_inv; auto with asmgen. rewrite Pregmap.gss; auto. rewrite <- EV; auto.
-(* intoffloat *)
-  apply SAME. TranslOp. rewrite H0; auto.
 (* floatofint *)
-  apply SAME. TranslOp. rewrite H0; auto.
-(* intofsingle *)
   apply SAME. TranslOp. rewrite H0; auto.
 (* singleofint *)
   apply SAME. TranslOp. rewrite H0; auto.
